@prefix : <https://w3id.org/def/och#> .
@prefix owl: <http://www.w3.org/2002/07/owl#> .
@prefix rdf: <http://www.w3.org/1999/02/22-rdf-syntax-ns#> .
@prefix xml: <http://www.w3.org/XML/1998/namespace> .
@prefix xsd: <http://www.w3.org/2001/XMLSchema#> .
@prefix rdfs: <http://www.w3.org/2000/01/rdf-schema#> .
@base <https://w3id.org/def/och#> .

<https://w3id.org/def/och#> rdf:type owl:Ontology ;
                             owl:versionIRI <http://w3id.org/def/och> ;
                             <http://creativecommons.org/ns#license> <http://creativecommons.org/publicdomain/zero/1.0/> ;
                             <http://purl.org/dc/terms/bibliographicCitation> "Conde-Herreros, D., Stork, L., Pernisch, R., Poveda-Villalón, M., Corcho, O., & Chaves-Fraga, D. (2024). Propagating Ontology Changes to Declarative Mappings in Construction of Knowledge Graphs." ;
                             <http://purl.org/dc/terms/contributor> "Diego Conde Herreros" ,
                                                                    "Raúl Palma" ;
                             <http://purl.org/dc/terms/created> "2024-04-17 "^^xsd:date ;
                             <http://purl.org/dc/terms/creator> "Diego Conde Herreros" ,
                                                                "Raúl Palma" ;
                             <http://purl.org/dc/terms/description> "An ontology for describing changes between OWL ontology versions" ;
                             <http://purl.org/dc/terms/title> "OWL Change Ontology" ;
                             <http://purl.org/vocab/vann/preferredNamespacePrefix> "och" ;
                             <http://purl.org/vocab/vann/preferredNamespaceUri> <https://w3id.org/def/och#> ;
                             owl:priorVersion <https://w3id.org/def/och#> .

#################################################################
#    Annotation properties
#################################################################

###  http://creativecommons.org/ns#license
<http://creativecommons.org/ns#license> rdf:type owl:AnnotationProperty .


###  http://purl.org/dc/terms/bibliographicCitation
<http://purl.org/dc/terms/bibliographicCitation> rdf:type owl:AnnotationProperty .


###  http://purl.org/dc/terms/contributor
<http://purl.org/dc/terms/contributor> rdf:type owl:AnnotationProperty .


###  http://purl.org/dc/terms/created
<http://purl.org/dc/terms/created> rdf:type owl:AnnotationProperty .


###  http://purl.org/dc/terms/creator
<http://purl.org/dc/terms/creator> rdf:type owl:AnnotationProperty .


###  http://purl.org/dc/terms/description
<http://purl.org/dc/terms/description> rdf:type owl:AnnotationProperty .


###  http://purl.org/dc/terms/title
<http://purl.org/dc/terms/title> rdf:type owl:AnnotationProperty .


###  http://purl.org/vocab/vann/preferredNamespacePrefix
<http://purl.org/vocab/vann/preferredNamespacePrefix> rdf:type owl:AnnotationProperty .


###  http://purl.org/vocab/vann/preferredNamespaceUri
<http://purl.org/vocab/vann/preferredNamespaceUri> rdf:type owl:AnnotationProperty .


#################################################################
#    Datatypes
#################################################################

###  http://www.w3.org/2001/XMLSchema#date
xsd:date rdf:type rdfs:Datatype .


#################################################################
#    Object Properties
#################################################################

###  https://w3id.orgdef/och#addedClass
<https://w3id.orgdef/och#addedClass> rdf:type owl:ObjectProperty ;
                                     rdfs:domain <https://w3id.orgdef/och#AddClass> ;
                                     rdfs:range owl:Class ;
                                     rdfs:comment "The OWL class that is added between ontology versions" ;
                                     rdfs:label "Added Class" .


###  https://w3id.orgdef/och#deprecatedElement
<https://w3id.orgdef/och#deprecatedElement> rdf:type owl:ObjectProperty ;
                                            rdfs:domain <https://w3id.orgdef/och#DeprecateElement> ;
                                            rdfs:range owl:Thing ;
                                            rdfs:comment "The Element that is being deprecated." ;
                                            rdfs:label "Deprecate Element" .


###  https://w3id.orgdef/och#domainAddDataProperty
<https://w3id.orgdef/och#domainAddDataProperty> rdf:type owl:ObjectProperty ;
                                                rdfs:domain <https://w3id.orgdef/och#AddDataProperty> ;
                                                rdfs:range owl:Class ;
                                                rdfs:comment "The domain of an OWL data property added between ontology versions" ;
                                                rdfs:label "Domain in Add Data Property" .


###  https://w3id.orgdef/och#domainAddObjectProperty
<https://w3id.orgdef/och#domainAddObjectProperty> rdf:type owl:ObjectProperty ;
                                                  rdfs:domain <https://w3id.orgdef/och#AddObjectProperty> ;
                                                  rdfs:range owl:Class ;
                                                  rdfs:comment "The domain of an OWL object property added between ontology versions" ;
                                                  rdfs:label "Domain in Add Object Property" .


###  https://w3id.orgdef/och#domainAddSubClass
<https://w3id.orgdef/och#domainAddSubClass> rdf:type owl:ObjectProperty ;
                                            rdfs:domain <https://w3id.orgdef/och#AddSubClass> ;
                                            rdfs:range owl:Class ;
                                            rdfs:comment "The subject of the rdfs:subClassOf property removed between ontology versions, the child class" ;
                                            rdfs:label "Domain in Add Subclass Property" .


###  https://w3id.orgdef/och#domainAddSubProperty
<https://w3id.orgdef/och#domainAddSubProperty> rdf:type owl:ObjectProperty ;
                                               rdfs:domain <https://w3id.orgdef/och#AddSubPropertyOf> ;
                                               rdfs:range owl:Property ;
                                               rdfs:comment "The subject of the rdfs:subPropertyOf property removed between ontology versions." ;
                                               rdfs:label "Domain in Add SubProperty Property" .


###  https://w3id.orgdef/och#domainRemoveDataProperty
<https://w3id.orgdef/och#domainRemoveDataProperty> rdf:type owl:ObjectProperty ;
                                                   rdfs:domain <https://w3id.orgdef/och#RemoveDataProperty> ;
                                                   rdfs:range owl:Class ;
                                                   rdfs:comment "The domain of an OWL data property removed between ontology versions" ;
                                                   rdfs:label "Domain in Remove Data Property" .


###  https://w3id.orgdef/och#domainRemoveObjectProperty
<https://w3id.orgdef/och#domainRemoveObjectProperty> rdf:type owl:ObjectProperty ;
                                                     rdfs:domain <https://w3id.orgdef/och#RemoveObjectProperty> ;
                                                     rdfs:range owl:Class ;
                                                     rdfs:comment "The domain of an OWL object property removed between ontology versions" ;
                                                     rdfs:label "Domain in Remove Object Property" .


###  https://w3id.orgdef/och#domainRemoveSubClass
<https://w3id.orgdef/och#domainRemoveSubClass> rdf:type owl:ObjectProperty ;
                                               rdfs:domain <https://w3id.orgdef/och#RemoveSubClass> ;
                                               rdfs:range owl:Class ;
                                               rdfs:comment "The subject of the rdfs:subClassOf property removed between ontology versions, the child class" ;
                                               rdfs:label "Domain in Remove Subclass Property" .


###  https://w3id.orgdef/och#domainRemoveSubProperty
<https://w3id.orgdef/och#domainRemoveSubProperty> rdf:type owl:ObjectProperty ;
                                                  rdfs:domain <https://w3id.orgdef/och#RemoveSubPropertyOf> ;
                                                  rdfs:range owl:Property ;
                                                  rdfs:comment "The subject of the rdfs:subPropertyOf property removed between ontology versions, the child class" ;
                                                  rdfs:label "Domain in Remove SubProperty Property" .


###  https://w3id.orgdef/och#hasRelatedEntity
<https://w3id.orgdef/och#hasRelatedEntity> rdf:type owl:ObjectProperty ;
                                           rdfs:domain <https://w3id.orgdef/och#OWLEntity> ;
                                           rdfs:range <https://w3id.orgdef/och#OWLEntity> ;
                                           rdfs:comment "EStablishes an equivalence between ontological terms" ;
                                           rdfs:label "Has Related Entity" .


###  https://w3id.orgdef/och#propertyAddDataProperty
<https://w3id.orgdef/och#propertyAddDataProperty> rdf:type owl:ObjectProperty ;
                                                  rdfs:domain <https://w3id.orgdef/och#AddDataProperty> ;
                                                  rdfs:range owl:DatatypeProperty ;
                                                  rdfs:comment "The data property added between ontology versions" ;
                                                  rdfs:label "Property in Add Data Property" .


###  https://w3id.orgdef/och#propertyAddObjectProperty
<https://w3id.orgdef/och#propertyAddObjectProperty> rdf:type owl:ObjectProperty ;
                                                    rdfs:domain <https://w3id.orgdef/och#AddObjectProperty> ;
                                                    rdfs:range owl:ObjectProperty ;
                                                    rdfs:comment "The object property added between ontology versions" ;
                                                    rdfs:label "Property in Add Object Property" .


###  https://w3id.orgdef/och#propertyRemoveDataProperty
<https://w3id.orgdef/och#propertyRemoveDataProperty> rdf:type owl:ObjectProperty ;
                                                     rdfs:domain <https://w3id.orgdef/och#RemoveDataProperty> ;
                                                     rdfs:range owl:DatatypeProperty ;
                                                     rdfs:comment "The data property removed between ontology versions" ;
                                                     rdfs:label "Property in Remove Data Property" .


###  https://w3id.orgdef/och#propertyRemoveObjectProperty
<https://w3id.orgdef/och#propertyRemoveObjectProperty> rdf:type owl:ObjectProperty ;
                                                       rdfs:domain <https://w3id.orgdef/och#RemoveObjectProperty> ;
                                                       rdfs:range owl:ObjectProperty ;
                                                       rdfs:comment "The data property removed between ontology versions" ;
                                                       rdfs:label "Property in Remove Data Property" .


###  https://w3id.orgdef/och#rangeAddObjectProperty
<https://w3id.orgdef/och#rangeAddObjectProperty> rdf:type owl:ObjectProperty ;
                                                 rdfs:domain <https://w3id.orgdef/och#AddObjectProperty> ;
                                                 rdfs:range owl:Class ;
                                                 rdfs:comment "The object of the object property added between ontology versions." ;
                                                 rdfs:label "Range in Add Object Property operation" .


###  https://w3id.orgdef/och#rangeAddSubClass
<https://w3id.orgdef/och#rangeAddSubClass> rdf:type owl:ObjectProperty ;
                                           rdfs:domain <https://w3id.orgdef/och#AddSubClass> ;
                                           rdfs:range owl:Class ;
                                           rdfs:comment "The object of the rdfs:subClassOf property added between ontology versions, the parent class." ;
                                           rdfs:label "Range in Add Subclass Property operation" .


###  https://w3id.orgdef/och#rangeAddSubProperty
<https://w3id.orgdef/och#rangeAddSubProperty> rdf:type owl:ObjectProperty ;
                                              rdfs:domain <https://w3id.orgdef/och#AddSubPropertyOf> ;
                                              rdfs:range owl:Property ;
                                              rdfs:comment "The object of the rdfs:subPropertyOf property removed between ontology versions." ;
                                              rdfs:label "Range in Add SubProperty Property" .


###  https://w3id.orgdef/och#rangeRemoveObjectProperty
<https://w3id.orgdef/och#rangeRemoveObjectProperty> rdf:type owl:ObjectProperty ;
                                                    rdfs:domain <https://w3id.orgdef/och#RemoveObjectProperty> ;
                                                    rdfs:range owl:Class ;
                                                    rdfs:comment "The range of an OWL object property removed between ontology versions" ;
                                                    rdfs:label "Range in Remove Object Property operation" .


###  https://w3id.orgdef/och#rangeRemoveSubClass
<https://w3id.orgdef/och#rangeRemoveSubClass> rdf:type owl:ObjectProperty ;
                                              rdfs:domain <https://w3id.orgdef/och#RemoveSubClass> ;
                                              rdfs:range owl:Class ;
                                              rdfs:comment "The object of the rdfs:subClassOf property removed between ontology versions, the parent class" ;
                                              rdfs:label "Range in Remove Subclass Property operation" .


###  https://w3id.orgdef/och#rangeRemoveSubProperty
<https://w3id.orgdef/och#rangeRemoveSubProperty> rdf:type owl:ObjectProperty ;
                                                 rdfs:domain <https://w3id.orgdef/och#RemoveSubPropertyOf> ;
                                                 rdfs:range owl:Property ;
                                                 rdfs:comment "The object of the rdfs:subPropertyOf property removed between ontology versions" ;
                                                 rdfs:label "Range in Remove SubProperty Property" .


###  https://w3id.orgdef/och#removedClass
<https://w3id.orgdef/och#removedClass> rdf:type owl:ObjectProperty ;
                                       rdfs:domain <https://w3id.orgdef/och#RemoveClass> ;
                                       rdfs:range owl:Class ;
                                       rdfs:comment "The OWL class that is deleted betweeen ontology versions" ;
                                       rdfs:label "Deleted Class" .


###  https://w3id.orgdef/och#renamedElement
<https://w3id.orgdef/och#renamedElement> rdf:type owl:ObjectProperty ;
                                         rdfs:domain <https://w3id.orgdef/och#RenameElement> ;
                                         rdfs:range owl:Thing ;
                                         rdfs:comment "The OWL class or property that is being renamed between ontology versions" ;
                                         rdfs:label "Renamed Element" .


###  https://w3id.orgdef/och#undeprecatedElement
<https://w3id.orgdef/och#undeprecatedElement> rdf:type owl:ObjectProperty ;
                                              rdfs:domain <https://w3id.orgdef/och#RevokeDeprecate> ;
                                              rdfs:range owl:Thing ;
                                              rdfs:comment "The Element that is being undeprecated." ;
                                              rdfs:label "Uneprecate Element" .


#################################################################
#    Data properties
#################################################################

###  https://w3id.orgdef/och#rangeAddDataProperty
<https://w3id.orgdef/och#rangeAddDataProperty> rdf:type owl:DatatypeProperty ;
                                               rdfs:domain <https://w3id.orgdef/och#AddDataProperty> ;
                                               rdfs:range rdfs:Literal ;
                                               rdfs:comment "The range of an OWL data property added between ontology versions" ;
                                               rdfs:label "Range in Add Data Property operation" .


###  https://w3id.orgdef/och#rangeRemoveDataProperty
<https://w3id.orgdef/och#rangeRemoveDataProperty> rdf:type owl:DatatypeProperty ;
                                                  rdfs:domain <https://w3id.orgdef/och#RemoveDataProperty> ;
                                                  rdfs:range rdfs:Literal ;
                                                  rdfs:comment "The range of an OWL data property removed between ontology versions" ;
                                                  rdfs:label "Range in Remove Data Property operation" .


#################################################################
#    Classes
#################################################################

###  http://www.w3.org/2002/07/owl#Class
owl:Class rdf:type owl:Class .


###  http://www.w3.org/2002/07/owl#DatatypeProperty
owl:DatatypeProperty rdf:type owl:Class .


###  http://www.w3.org/2002/07/owl#ObjectProperty
owl:ObjectProperty rdf:type owl:Class .


###  http://www.w3.org/2002/07/owl#Property
owl:Property rdf:type owl:Class .


###  https://w3id.orgdef/och#AddAsymmetricObjectProperty
<https://w3id.orgdef/och#AddAsymmetricObjectProperty> rdf:type owl:Class ;
                                                      rdfs:subClassOf <https://w3id.orgdef/och#AddObjectProperty> ,
                                                                      <https://w3id.orgdef/och#AsymmetricObjectPropertyChange> ;
                                                      rdfs:comment "The class of the addition of asymmetric properties change betweeen ontology versions" ;
                                                      rdfs:label "Addition of Asymetric Object Property" .


###  https://w3id.orgdef/och#AddClass
<https://w3id.orgdef/och#AddClass> rdf:type owl:Class ;
                                   rdfs:subClassOf <https://w3id.orgdef/och#ClassChange> ;
                                   rdfs:comment "The addition of a class operation" ;
                                   rdfs:label "Addition of Class" .


###  https://w3id.orgdef/och#AddDataProperty
<https://w3id.orgdef/och#AddDataProperty> rdf:type owl:Class ;
                                          rdfs:subClassOf <https://w3id.orgdef/och#AddProperty> ,
                                                          <https://w3id.orgdef/och#DataPropertyChange> ;
                                          rdfs:comment "The class of the addition of data properties change betweeen ontology versions" ;
                                          rdfs:label "Addition of Data Property" .


###  https://w3id.orgdef/och#AddDataPropertyDomain
<https://w3id.orgdef/och#AddDataPropertyDomain> rdf:type owl:Class ;
                                                rdfs:subClassOf <https://w3id.orgdef/och#AddDomain> ,
                                                                <https://w3id.orgdef/och#DataPropertyDomainChange> ;
                                                rdfs:comment "The class of the addition of the domain of a data property change betweeen ontology versions" ;
                                                rdfs:label "Addition of the Domain of a Data Property" .


###  https://w3id.orgdef/och#AddDataPropertyRange
<https://w3id.orgdef/och#AddDataPropertyRange> rdf:type owl:Class ;
                                               rdfs:subClassOf <https://w3id.orgdef/och#AddRange> ,
                                                               <https://w3id.orgdef/och#DataPropertyRangeChange> ;
                                               rdfs:comment "The class of the addition of the range of a data property change betweeen ontology versions" ;
                                               rdfs:label "Addition of the Range of a Data Property" .


###  https://w3id.orgdef/och#AddDatatype
<https://w3id.orgdef/och#AddDatatype> rdf:type owl:Class ;
                                      rdfs:subClassOf <https://w3id.orgdef/och#DatatypeChange> ;
                                      rdfs:comment "The class of the addition of the Datatype of a data property change betweeen ontology versions" ;
                                      rdfs:label "Addition of the Datatype of a Data Property" .


###  https://w3id.orgdef/och#AddDisjointClass
<https://w3id.orgdef/och#AddDisjointClass> rdf:type owl:Class ;
                                           rdfs:subClassOf <https://w3id.orgdef/och#DisjointClassChange> ;
                                           rdfs:comment "The class of the addition of the owl:disjointWith property change betweeen ontology versions" ;
                                           rdfs:label "Addition of the Disjoint With Property" .


###  https://w3id.orgdef/och#AddDisjointDataProperty
<https://w3id.orgdef/och#AddDisjointDataProperty> rdf:type owl:Class ;
                                                  rdfs:subClassOf <https://w3id.orgdef/och#DisjointDataPropertyChange> ;
                                                  rdfs:comment "The class of the addition of the owl:propertyDisjointWith property betweeen data properties change betweeen ontology versions" ;
                                                  rdfs:label "Addition of the property Disjoint With Property to data property" .


###  https://w3id.orgdef/och#AddDisjointObjectProperty
<https://w3id.orgdef/och#AddDisjointObjectProperty> rdf:type owl:Class ;
                                                    rdfs:subClassOf <https://w3id.orgdef/och#AddProperty> ,
                                                                    <https://w3id.orgdef/och#DisjointObjectPropertyChange> ;
                                                    rdfs:comment "The class of the addition of the owl:propertyDisjointWith property betweeen object properties change betweeen ontology versions" ;
                                                    rdfs:label "Addition of the property Disjoint With Property to object property" .


###  https://w3id.orgdef/och#AddDisjointUnion
<https://w3id.orgdef/och#AddDisjointUnion> rdf:type owl:Class ;
                                           rdfs:subClassOf <https://w3id.orgdef/och#DisjointUnionChange> ;
                                           rdfs:comment "The class of the addition of the owl:DisjointUnionOf property change betweeen ontology versions. The property that determines that a given class is equivalent to the disjoint union of a collection of other classes" ;
                                           rdfs:label "Addition of the DisjointUnionOf Property" .


###  https://w3id.orgdef/och#AddDomain
<https://w3id.orgdef/och#AddDomain> rdf:type owl:Class ;
                                    rdfs:subClassOf <https://w3id.orgdef/och#DomainChange> ;
                                    rdfs:comment "The change operation that describes the addition of a domain to a property." ;
                                    rdfs:label "Addition of the Domain" .


###  https://w3id.orgdef/och#AddEquivalentClass
<https://w3id.orgdef/och#AddEquivalentClass> rdf:type owl:Class ;
                                             rdfs:subClassOf <https://w3id.orgdef/och#EquivalentClassChange> ;
                                             rdfs:comment "The class of the addition of the owl:equivalentClass property change betweeen ontology versions. The property that determines that two given classes are equivalent, and that is used to specify datatype definitions." ;
                                             rdfs:label "Addition of the equivalentClass Property" .


###  https://w3id.orgdef/och#AddEquivalentDataProperty
<https://w3id.orgdef/och#AddEquivalentDataProperty> rdf:type owl:Class ;
                                                    rdfs:subClassOf <https://w3id.orgdef/och#EquivalentDataPropertyChange> ;
                                                    rdfs:comment "The class of the addition of the owl:equivalentProperty property between data properties change betweeen ontology versions. The property that determines that two given properties are equivalent." ;
                                                    rdfs:label "Addition of the equivalentProperty Property for data properties" .


###  https://w3id.orgdef/och#AddEquivalentObjectProperty
<https://w3id.orgdef/och#AddEquivalentObjectProperty> rdf:type owl:Class ;
                                                      rdfs:subClassOf <https://w3id.orgdef/och#AddObjectProperty> ,
                                                                      <https://w3id.orgdef/och#EquivalentObjectPropertyChange> ;
                                                      rdfs:comment "The class of the addition of the owl:equivalentProperty property between object properties change betweeen ontology versions. The property that determines that two given properties are equivalent." ;
                                                      rdfs:label "Addition of the equivalentProperty Property for object properties" .


###  https://w3id.orgdef/och#AddFunctionalDataProperty
<https://w3id.orgdef/och#AddFunctionalDataProperty> rdf:type owl:Class ;
                                                    rdfs:subClassOf <https://w3id.orgdef/och#FunctionalDataPropertyChange> ;
                                                    rdfs:comment "The class of the addition of the owl:FuctionalProperty change betweeen ontology versions.This is the class of functional properties" ;
                                                    rdfs:label "Addition of functional data property " .


###  https://w3id.orgdef/och#AddFunctionalObjectProperty
<https://w3id.orgdef/och#AddFunctionalObjectProperty> rdf:type owl:Class ;
                                                      rdfs:subClassOf <https://w3id.orgdef/och#AddProperty> ,
                                                                      <https://w3id.orgdef/och#FunctionalObjectPropertyChange> ;
                                                      rdfs:comment "The class of the addition of the owl:FuctionalProperty change betweeen ontology versions.This is the class of functional properties" ;
                                                      rdfs:label "Addition of Functional Object Property" .


###  https://w3id.orgdef/och#AddInverseFunctionalObjectProperty
<https://w3id.orgdef/och#AddInverseFunctionalObjectProperty> rdf:type owl:Class ;
                                                             rdfs:subClassOf <https://w3id.orgdef/och#AddObjectProperty> ,
                                                                             <https://w3id.orgdef/och#InverseFunctionalObjectPropertyChange> ;
                                                             rdfs:comment "The class of the addition of the owl:InverseFuctionalProperty change betweeen ontology versions.This is the class of inverse-functional properties" ;
                                                             rdfs:label "Addition of an inverse functional object property " .


###  https://w3id.orgdef/och#AddInverseObjectProperty
<https://w3id.orgdef/och#AddInverseObjectProperty> rdf:type owl:Class ;
                                                   rdfs:subClassOf <https://w3id.orgdef/och#AddObjectProperty> ,
                                                                   <https://w3id.orgdef/och#InverseObjectPropertyChange> ;
                                                   rdfs:comment "The class of the addition of the owl:inverseOf change betweeen ontology versions.The property that determines that two given properties are inverse." ;
                                                   rdfs:label "Addition of an inverse property to object property " .


###  https://w3id.orgdef/och#AddIrreflexiveObjectProperty
<https://w3id.orgdef/och#AddIrreflexiveObjectProperty> rdf:type owl:Class ;
                                                       rdfs:subClassOf <https://w3id.orgdef/och#AddObjectProperty> ,
                                                                       <https://w3id.orgdef/och#IrreflexiveObjectPropertyChange> ;
                                                       rdfs:comment "The class of the addition of the owl:irreflexiveProperty change betweeen ontology versions.The class of irreflexive properties." ;
                                                       rdfs:label "Addition of an irreflexive object property " .


###  https://w3id.orgdef/och#AddObjectProperty
<https://w3id.orgdef/och#AddObjectProperty> rdf:type owl:Class ;
                                            rdfs:subClassOf <https://w3id.orgdef/och#AddProperty> ,
                                                            <https://w3id.orgdef/och#ObjectPropertyChange> ;
                                            rdfs:comment "Addition of an Object type property." ;
                                            rdfs:label "Addition of an Object property" .


###  https://w3id.orgdef/och#AddObjectPropertyDomain
<https://w3id.orgdef/och#AddObjectPropertyDomain> rdf:type owl:Class ;
                                                  rdfs:subClassOf <https://w3id.orgdef/och#AddDomain> ,
                                                                  <https://w3id.orgdef/och#ObjectPropertyDomainChange> ;
                                                  rdfs:comment "The class of the addition of the domain of an object property change betweeen ontology versions" ;
                                                  rdfs:label "Addition of the Domain of an object property" .


###  https://w3id.orgdef/och#AddObjectPropertyRange
<https://w3id.orgdef/och#AddObjectPropertyRange> rdf:type owl:Class ;
                                                 rdfs:subClassOf <https://w3id.orgdef/och#AddRange> ,
                                                                 <https://w3id.orgdef/och#ObjectPropertyRangeChange> ;
                                                 rdfs:comment "The class of the addition of the range of an object property change betweeen ontology versions" ;
                                                 rdfs:label "Addition of the Range of an object property" .


###  https://w3id.orgdef/och#AddProperty
<https://w3id.orgdef/och#AddProperty> rdf:type owl:Class ;
                                      rdfs:subClassOf <https://w3id.orgdef/och#PropertyChange> ;
                                      rdfs:comment "The change operation that describes the addition of a property to the ontology." ;
                                      rdfs:label "Addition of a Property" .


###  https://w3id.orgdef/och#AddRange
<https://w3id.orgdef/och#AddRange> rdf:type owl:Class ;
                                   rdfs:subClassOf <https://w3id.orgdef/och#RangeChange> ;
                                   rdfs:comment "The change operation that describes the addition of a range to a property." ;
                                   rdfs:label "Addition of the Range" .


###  https://w3id.orgdef/och#AddReflexiveObjectProperty
<https://w3id.orgdef/och#AddReflexiveObjectProperty> rdf:type owl:Class ;
                                                     rdfs:subClassOf <https://w3id.orgdef/och#AddObjectProperty> ,
                                                                     <https://w3id.orgdef/och#ReflexiveObjectPropertyChange> ;
                                                     rdfs:comment "The class of the addition of the owl:reflexiveProperty change betweeen ontology versions.The class of rreflexive properties." ;
                                                     rdfs:label "Addition of an reflexive object property " .


###  https://w3id.orgdef/och#AddSubClass
<https://w3id.orgdef/och#AddSubClass> rdf:type owl:Class ;
                                      rdfs:subClassOf <https://w3id.orgdef/och#SubClassChange> ;
                                      rdfs:comment "The change operation that describes the addition of an rdfs:subClassOf property." ;
                                      rdfs:label "Addition  of SubClass property" .


###  https://w3id.orgdef/och#AddSubPropertyOf
<https://w3id.orgdef/och#AddSubPropertyOf> rdf:type owl:Class ;
                                           rdfs:subClassOf <https://w3id.orgdef/och#SubPropertyChange> ;
                                           rdfs:comment "The change operation that describes the addition of sub property property." ;
                                           rdfs:label "Addition of the sub-property property" .


###  https://w3id.orgdef/och#AddSymmetricObjectProperty
<https://w3id.orgdef/och#AddSymmetricObjectProperty> rdf:type owl:Class ;
                                                     rdfs:subClassOf <https://w3id.orgdef/och#AddObjectProperty> ,
                                                                     <https://w3id.orgdef/och#SymmetricObjectPropertyChange> ;
                                                     rdfs:comment "The change operation that describes the addition of Symmetric object property." ;
                                                     rdfs:label "Addition a Symmetric object property" .


###  https://w3id.orgdef/och#AddTransitiveObjectProperty
<https://w3id.orgdef/och#AddTransitiveObjectProperty> rdf:type owl:Class ;
                                                      rdfs:subClassOf <https://w3id.orgdef/och#AddObjectProperty> ,
                                                                      <https://w3id.orgdef/och#TransitiveObjectPropertyChange> ;
                                                      rdfs:comment "The change operation that describes the addition of a transitive object property." ;
                                                      rdfs:label "Addition a transitive object property" .


###  https://w3id.orgdef/och#AsymmetricObjectPropertyChange
<https://w3id.orgdef/och#AsymmetricObjectPropertyChange> rdf:type owl:Class ;
                                                         rdfs:subClassOf <https://w3id.orgdef/och#ObjectPropertyChange> ;
                                                         rdfs:comment "The change operation that describes the change of a transitive object property." ;
                                                         rdfs:label "Change of an asymmetric object property" .


###  https://w3id.orgdef/och#ClassChange
<https://w3id.orgdef/och#ClassChange> rdf:type owl:Class ;
                                      rdfs:subClassOf <https://w3id.orgdef/och#OntologyChange> ;
                                      rdfs:comment "The change operation that describes changes in classes." ;
                                      rdfs:label "Class Changes" .


###  https://w3id.orgdef/och#DataPropertyChange
<https://w3id.orgdef/och#DataPropertyChange> rdf:type owl:Class ;
                                             rdfs:subClassOf <https://w3id.orgdef/och#PropertyChange> ;
                                             rdfs:comment "The change operation that describes the change of a datatype property." ;
                                             rdfs:label "Change of a Datatype Property" .


###  https://w3id.orgdef/och#DataPropertyDomainChange
<https://w3id.orgdef/och#DataPropertyDomainChange> rdf:type owl:Class ;
                                                   rdfs:subClassOf <https://w3id.orgdef/och#DataPropertyChange> ;
                                                   rdfs:comment "The change operation that describes the change of  the domain of a datatype property." ;
                                                   rdfs:label "Change of  the Domain of a Datatype Property" .


###  https://w3id.orgdef/och#DataPropertyRangeChange
<https://w3id.orgdef/och#DataPropertyRangeChange> rdf:type owl:Class ;
                                                  rdfs:subClassOf <https://w3id.orgdef/och#DataPropertyChange> ;
                                                  rdfs:comment "The change operation that describes the change of  the range of a datatype property." ;
                                                  rdfs:label "Change of  the range of a datatype property" .


###  https://w3id.orgdef/och#DatatypeChange
<https://w3id.orgdef/och#DatatypeChange> rdf:type owl:Class ;
                                         rdfs:subClassOf <https://w3id.orgdef/och#DataPropertyChange> ;
                                         rdfs:comment "The change operation that describes the change of the datatype of a property" ;
                                         rdfs:label "Change of the Datatype of a Property" .


###  https://w3id.orgdef/och#DeprecateElement
<https://w3id.orgdef/och#DeprecateElement> rdf:type owl:Class ;
                                           rdfs:subClassOf <https://w3id.orgdef/och#ElementChange> ;
                                           rdfs:comment "The change operation that describes the deprecation of a class or property" ;
                                           rdfs:label "Deprecation of an element." .


###  https://w3id.orgdef/och#DisjointClassChange
<https://w3id.orgdef/och#DisjointClassChange> rdf:type owl:Class ;
                                              rdfs:subClassOf <https://w3id.orgdef/och#ClassChange> ;
                                              rdfs:comment "The change operation that describes the change of a disjoint class." ;
                                              rdfs:label "Change of a disjoint class" .


###  https://w3id.orgdef/och#DisjointDataPropertyChange
<https://w3id.orgdef/och#DisjointDataPropertyChange> rdf:type owl:Class ;
                                                     rdfs:subClassOf <https://w3id.orgdef/och#DataPropertyChange> ;
                                                     rdfs:comment "The change operation that describes the change of a disjoint datatype property." ;
                                                     rdfs:label "Change of a Disjoint datatype property" .


###  https://w3id.orgdef/och#DisjointObjectPropertyChange
<https://w3id.orgdef/och#DisjointObjectPropertyChange> rdf:type owl:Class ;
                                                       rdfs:subClassOf <https://w3id.orgdef/och#ObjectPropertyChange> ;
                                                       rdfs:comment "The change operation that describes the change of a disjoint object property." ;
                                                       rdfs:label "Change of a Disjoint Object Property" .


###  https://w3id.orgdef/och#DisjointUnionChange
<https://w3id.orgdef/och#DisjointUnionChange> rdf:type owl:Class ;
                                              rdfs:subClassOf <https://w3id.orgdef/och#ClassChange> ;
                                              rdfs:comment "The change operation that describes the change of a disjoint union property." ;
                                              rdfs:label "Change of a disjoint union property" .


###  https://w3id.orgdef/och#DomainChange
<https://w3id.orgdef/och#DomainChange> rdf:type owl:Class ;
                                       rdfs:subClassOf <https://w3id.orgdef/och#PropertyChange> ;
                                       rdfs:comment "Change operation that describes the change of the domain of a property" ;
                                       rdfs:label "Change of the domain of a property" .


###  https://w3id.orgdef/och#ElementChange
<https://w3id.orgdef/och#ElementChange> rdf:type owl:Class ;
                                        rdfs:subClassOf <https://w3id.orgdef/och#OntologyChange> ;
                                        rdfs:comment "The change operation that describes changes in changes and properties." ;
                                        rdfs:label "Element Changes" .


###  https://w3id.orgdef/och#EquivalentClassChange
<https://w3id.orgdef/och#EquivalentClassChange> rdf:type owl:Class ;
                                                rdfs:subClassOf <https://w3id.orgdef/och#ClassChange> ;
                                                rdfs:comment "The change operation that describes the change of an equivalent class property." ;
                                                rdfs:label "Change of an equivalent class property" .


###  https://w3id.orgdef/och#EquivalentDataPropertyChange
<https://w3id.orgdef/och#EquivalentDataPropertyChange> rdf:type owl:Class ;
                                                       rdfs:subClassOf <https://w3id.orgdef/och#DataPropertyChange> ;
                                                       rdfs:comment "The change operation that describes the change of an equivalent data property property." ;
                                                       rdfs:label "Change of an Equivalent Data Property property" .


###  https://w3id.orgdef/och#EquivalentObjectPropertyChange
<https://w3id.orgdef/och#EquivalentObjectPropertyChange> rdf:type owl:Class ;
                                                         rdfs:subClassOf <https://w3id.orgdef/och#ObjectPropertyChange> ;
                                                         rdfs:comment "The change operation that describes the change of an equivalent object property property." ;
                                                         rdfs:label "Change of an equivalent object property property" .


###  https://w3id.orgdef/och#FunctionalDataPropertyChange
<https://w3id.orgdef/och#FunctionalDataPropertyChange> rdf:type owl:Class ;
                                                       rdfs:subClassOf <https://w3id.orgdef/och#DataPropertyChange> ;
                                                       rdfs:comment "The change operation that describes the change of a functional datatype property property." ;
                                                       rdfs:label "Change of a Functional Datatype Property property" .


###  https://w3id.orgdef/och#FunctionalObjectPropertyChange
<https://w3id.orgdef/och#FunctionalObjectPropertyChange> rdf:type owl:Class ;
                                                         rdfs:subClassOf <https://w3id.orgdef/och#ObjectPropertyChange> ,
                                                                         <https://w3id.orgdef/och#RemoveObjectProperty> ;
                                                         rdfs:comment "The change operation that describes the change of a functional object property property." ;
                                                         rdfs:label "Change of a Functional Object Property property" .


###  https://w3id.orgdef/och#InverseFunctionalObjectPropertyChange
<https://w3id.orgdef/och#InverseFunctionalObjectPropertyChange> rdf:type owl:Class ;
                                                                rdfs:subClassOf <https://w3id.orgdef/och#ObjectPropertyChange> ;
                                                                rdfs:comment "The change operation that describes the change of an inverse functional object property property." ;
                                                                rdfs:label "Change of an inverse functional object property property" .


###  https://w3id.orgdef/och#InverseObjectPropertyChange
<https://w3id.orgdef/och#InverseObjectPropertyChange> rdf:type owl:Class ;
                                                      rdfs:subClassOf <https://w3id.orgdef/och#ObjectPropertyChange> ;
                                                      rdfs:comment "The change operation that describes the change of an inverse functional object property property." ;
                                                      rdfs:label "Change of an inverse functional object property property" .


###  https://w3id.orgdef/och#IrreflexiveObjectPropertyChange
<https://w3id.orgdef/och#IrreflexiveObjectPropertyChange> rdf:type owl:Class ;
                                                          rdfs:subClassOf <https://w3id.orgdef/och#ObjectPropertyChange> ;
                                                          rdfs:comment "The change operation that describes the change of an irreflexive object property property." ;
                                                          rdfs:label "Change of an irreflexive object property property" .


###  https://w3id.orgdef/och#OWLEntity
<https://w3id.orgdef/och#OWLEntity> rdf:type owl:Class ;
                                    rdfs:comment "The class that describes an OWL Entities, the named terms of the ontology" ;
                                    rdfs:label "OWL Entity Class" .


###  https://w3id.orgdef/och#ObjectPropertyChange
<https://w3id.orgdef/och#ObjectPropertyChange> rdf:type owl:Class ;
                                               rdfs:subClassOf <https://w3id.orgdef/och#PropertyChange> ;
                                               rdfs:comment "The change operation that describes the change of an object property." ;
                                               rdfs:label "Change of an Object Property" .


###  https://w3id.orgdef/och#ObjectPropertyDomainChange
<https://w3id.orgdef/och#ObjectPropertyDomainChange> rdf:type owl:Class ;
                                                     rdfs:subClassOf <https://w3id.orgdef/och#ObjectPropertyChange> ;
                                                     rdfs:comment "The change operation that describes the change of the domain of an object property." ;
                                                     rdfs:label "Change of the domain of an object property" .


###  https://w3id.orgdef/och#ObjectPropertyRangeChange
<https://w3id.orgdef/och#ObjectPropertyRangeChange> rdf:type owl:Class ;
                                                    rdfs:subClassOf <https://w3id.orgdef/och#ObjectPropertyChange> ;
                                                    rdfs:comment "The change operation that describes the change of the range of an object property." ;
                                                    rdfs:label "Change of the range of an object property" .


###  https://w3id.orgdef/och#OntologyChange
<https://w3id.orgdef/och#OntologyChange> rdf:type owl:Class ;
                                         rdfs:comment "The change operation that describes changes in an ontology." ;
                                         rdfs:label "Ontology Changes" .


###  https://w3id.orgdef/och#PropertyChange
<https://w3id.orgdef/och#PropertyChange> rdf:type owl:Class ;
                                         rdfs:subClassOf <https://w3id.orgdef/och#OntologyChange> ;
                                         rdfs:comment "The change operation that describes changes in properties." ;
                                         rdfs:label "Property Changes" .


###  https://w3id.orgdef/och#RangeChange
<https://w3id.orgdef/och#RangeChange> rdf:type owl:Class ;
                                      rdfs:subClassOf <https://w3id.orgdef/och#PropertyChange> ;
                                      rdfs:comment "The change operation that describes the change of the range of a property" ;
                                      rdfs:label "Change of the range of a property" .


###  https://w3id.orgdef/och#ReflexiveObjectPropertyChange
<https://w3id.orgdef/och#ReflexiveObjectPropertyChange> rdf:type owl:Class ;
                                                        rdfs:subClassOf <https://w3id.orgdef/och#ObjectPropertyChange> ;
                                                        rdfs:comment "The change operation that describes the change a reflexive object property." ;
                                                        rdfs:label "Change of a reflexive object property" .


###  https://w3id.orgdef/och#RemoveAsymmetricObjectProperty
<https://w3id.orgdef/och#RemoveAsymmetricObjectProperty> rdf:type owl:Class ;
                                                         rdfs:subClassOf <https://w3id.orgdef/och#AsymmetricObjectPropertyChange> ,
                                                                         <https://w3id.orgdef/och#RemoveObjectProperty> ;
                                                         rdfs:comment "The change operation that describes the removal of an asymmetric object property." ;
                                                         rdfs:label "Removal of an asymmetric object property" .


###  https://w3id.orgdef/och#RemoveClass
<https://w3id.orgdef/och#RemoveClass> rdf:type owl:Class ;
                                      rdfs:subClassOf <https://w3id.orgdef/och#ClassChange> ;
                                      rdfs:comment "The change operation that describes the removal of a class." ;
                                      rdfs:label "Removal of a class" .


###  https://w3id.orgdef/och#RemoveDataProperty
<https://w3id.orgdef/och#RemoveDataProperty> rdf:type owl:Class ;
                                             rdfs:subClassOf <https://w3id.orgdef/och#DataPropertyChange> ,
                                                             <https://w3id.orgdef/och#RemoveProperty> ;
                                             rdfs:comment "The change operation that describes the removal of a data property." ;
                                             rdfs:label "Removal of a Data Property" .


###  https://w3id.orgdef/och#RemoveDataPropertyDomain
<https://w3id.orgdef/och#RemoveDataPropertyDomain> rdf:type owl:Class ;
                                                   rdfs:subClassOf <https://w3id.orgdef/och#DataPropertyDomainChange> ,
                                                                   <https://w3id.orgdef/och#RemoveDomain> ;
                                                   rdfs:comment "The change operation that describes the removal of the domain of a data property." ;
                                                   rdfs:label "Removal of the domain of a datatype property" .


###  https://w3id.orgdef/och#RemoveDataPropertyRange
<https://w3id.orgdef/och#RemoveDataPropertyRange> rdf:type owl:Class ;
                                                  rdfs:subClassOf <https://w3id.orgdef/och#DataPropertyRangeChange> ,
                                                                  <https://w3id.orgdef/och#RemoveRange> ;
                                                  rdfs:comment "The change operation that describes the removal of the range of a data property." ;
                                                  rdfs:label "Removal of the range of a datatype property" .


###  https://w3id.orgdef/och#RemoveDatatype
<https://w3id.orgdef/och#RemoveDatatype> rdf:type owl:Class ;
                                         rdfs:subClassOf <https://w3id.orgdef/och#DatatypeChange> ;
                                         rdfs:comment "The change operation that describes the removal of the Datatype of a data property." ;
                                         rdfs:label "Removal of the Datatype of a Datatype Property" .


###  https://w3id.orgdef/och#RemoveDisjointClass
<https://w3id.orgdef/och#RemoveDisjointClass> rdf:type owl:Class ;
                                              rdfs:subClassOf <https://w3id.orgdef/och#DisjointClassChange> ;
                                              rdfs:comment "The change operation that describes the removal of the disjoint class property." ;
                                              rdfs:label "Removal of a disjoint class property" .


###  https://w3id.orgdef/och#RemoveDisjointDataProperty
<https://w3id.orgdef/och#RemoveDisjointDataProperty> rdf:type owl:Class ;
                                                     rdfs:subClassOf <https://w3id.orgdef/och#DisjointDataPropertyChange> ;
                                                     rdfs:comment "The change operation that describes the removal of the disjointWith property." ;
                                                     rdfs:label "Removal of the disjointWith property" .


###  https://w3id.orgdef/och#RemoveDisjointObjectProperty
<https://w3id.orgdef/och#RemoveDisjointObjectProperty> rdf:type owl:Class ;
                                                       rdfs:subClassOf <https://w3id.orgdef/och#DisjointObjectPropertyChange> ,
                                                                       <https://w3id.orgdef/och#RemoveObjectProperty> ;
                                                       rdfs:comment "The change operation that describes the removal of the disjointWith property." ;
                                                       rdfs:label "Removal of the disjointWith property" .


###  https://w3id.orgdef/och#RemoveDisjointUnion
<https://w3id.orgdef/och#RemoveDisjointUnion> rdf:type owl:Class ;
                                              rdfs:subClassOf <https://w3id.orgdef/och#DisjointUnionChange> ;
                                              rdfs:comment "The change operation that describes the removal of the disjointUnionOf property." ;
                                              rdfs:label "Removal of the disjointUnionOf property" .


###  https://w3id.orgdef/och#RemoveDomain
<https://w3id.orgdef/och#RemoveDomain> rdf:type owl:Class ;
                                       rdfs:subClassOf <https://w3id.orgdef/och#DomainChange> ;
                                       rdfs:comment "The change operation that describes the removal of the domain from a property." ;
                                       rdfs:label "Removal of the Domain" .


###  https://w3id.orgdef/och#RemoveEquivalentClass
<https://w3id.orgdef/och#RemoveEquivalentClass> rdf:type owl:Class ;
                                                rdfs:subClassOf <https://w3id.orgdef/och#EquivalentClassChange> ;
                                                rdfs:comment "The change operation that describes the removal of the equivalentClass property." ;
                                                rdfs:label "Removal of the equivalentClass property" .


###  https://w3id.orgdef/och#RemoveEquivalentDataProperty
<https://w3id.orgdef/och#RemoveEquivalentDataProperty> rdf:type owl:Class ;
                                                       rdfs:subClassOf <https://w3id.orgdef/och#EquivalentDataPropertyChange> ;
                                                       rdfs:comment "The change operation that describes the removal of the equivalentProperty property for a Datatype property." ;
                                                       rdfs:label "Removal of the equivalentProperty property for a Datatype property" .


###  https://w3id.orgdef/och#RemoveEquivalentObjectProperty
<https://w3id.orgdef/och#RemoveEquivalentObjectProperty> rdf:type owl:Class ;
                                                         rdfs:subClassOf <https://w3id.orgdef/och#EquivalentObjectPropertyChange> ,
                                                                         <https://w3id.orgdef/och#RemoveObjectProperty> ;
                                                         rdfs:comment "The change operation that describes the removal of the equivalentProperty property for an object property." ;
                                                         rdfs:label "Removal of the equivalentProperty property for an object property" .


###  https://w3id.orgdef/och#RemoveFunctionalDataProperty
<https://w3id.orgdef/och#RemoveFunctionalDataProperty> rdf:type owl:Class ;
                                                       rdfs:subClassOf <https://w3id.orgdef/och#FunctionalDataPropertyChange> ;
                                                       rdfs:comment "The class of the removal of the owl:FuctionalProperty change betweeen ontology versions.This is the class of functional properties" ;
                                                       rdfs:label "Removal of functional data property " .


###  https://w3id.orgdef/och#RemoveFunctionalObjectProperty
<https://w3id.orgdef/och#RemoveFunctionalObjectProperty> rdf:type owl:Class ;
                                                         rdfs:subClassOf <https://w3id.orgdef/och#FunctionalObjectPropertyChange> ;
                                                         rdfs:comment "The class of the removal of the owl:InverseFuctionalProperty change betweeen ontology versions.This is the class of inverse functional properties" ;
                                                         rdfs:label "Removal of functional object property " .


###  https://w3id.orgdef/och#RemoveInverseFunctionalObjectProperty
<https://w3id.orgdef/och#RemoveInverseFunctionalObjectProperty> rdf:type owl:Class ;
                                                                rdfs:subClassOf <https://w3id.orgdef/och#InverseFunctionalObjectPropertyChange> ,
                                                                                <https://w3id.orgdef/och#RemoveObjectProperty> ;
                                                                rdfs:comment "The class of the removal of the owl:InverseFuctionalProperty change betweeen ontology versions.This is the class of inverse functional properties" ;
                                                                rdfs:label "Removal of inverse functional object property " .


###  https://w3id.orgdef/och#RemoveInverseObjectProperty
<https://w3id.orgdef/och#RemoveInverseObjectProperty> rdf:type owl:Class ;
                                                      rdfs:subClassOf <https://w3id.orgdef/och#InverseObjectPropertyChange> ,
                                                                      <https://w3id.orgdef/och#RemoveObjectProperty> ;
                                                      rdfs:comment "The class of the removal of the owl:inverseOf change betweeen ontology versions.The property that determines that two given properties are inverse." ;
                                                      rdfs:label "Removal of an inverse property to object property " .


###  https://w3id.orgdef/och#RemoveIrreflexiveObjectProperty
<https://w3id.orgdef/och#RemoveIrreflexiveObjectProperty> rdf:type owl:Class ;
                                                          rdfs:subClassOf <https://w3id.orgdef/och#IrreflexiveObjectPropertyChange> ;
                                                          rdfs:comment "The class of the removal of the owl:irreflexiveProperty change betweeen ontology versions.The class of irreflexive properties." ;
                                                          rdfs:label "Removal of an irreflexive object property " .


###  https://w3id.orgdef/och#RemoveObjectProperty
<https://w3id.orgdef/och#RemoveObjectProperty> rdf:type owl:Class ;
                                               rdfs:subClassOf <https://w3id.orgdef/och#ObjectPropertyChange> ,
                                                               <https://w3id.orgdef/och#RemoveProperty> ;
                                               rdfs:comment "Removal of an Object type property." ;
                                               rdfs:label "Removal of an Object property" .


###  https://w3id.orgdef/och#RemoveObjectPropertyDomain
<https://w3id.orgdef/och#RemoveObjectPropertyDomain> rdf:type owl:Class ;
                                                     rdfs:subClassOf <https://w3id.orgdef/och#ObjectPropertyDomainChange> ,
                                                                     <https://w3id.orgdef/och#RemoveDomain> ;
                                                     rdfs:comment "The class of the removal of the domain of an object property change betweeen ontology versions" ;
                                                     rdfs:label "Removal of the Domain of an object property" .


###  https://w3id.orgdef/och#RemoveObjectPropertyRange
<https://w3id.orgdef/och#RemoveObjectPropertyRange> rdf:type owl:Class ;
                                                    rdfs:subClassOf <https://w3id.orgdef/och#ObjectPropertyRangeChange> ,
                                                                    <https://w3id.orgdef/och#RemoveRange> ;
                                                    rdfs:comment "The class of the removal of the range of an object property change betweeen ontology versions" ;
                                                    rdfs:label "Removal of the Range of an object property" .


###  https://w3id.orgdef/och#RemoveProperty
<https://w3id.orgdef/och#RemoveProperty> rdf:type owl:Class ;
                                         rdfs:subClassOf <https://w3id.orgdef/och#PropertyChange> ;
                                         rdfs:comment "The change operation that describes the removal of a Property." ;
                                         rdfs:label "Removal of a Property" .


###  https://w3id.orgdef/och#RemoveRange
<https://w3id.orgdef/och#RemoveRange> rdf:type owl:Class ;
                                      rdfs:subClassOf <https://w3id.orgdef/och#RangeChange> ;
                                      rdfs:comment "The change operation that describes the removal of the range from a property." ;
                                      rdfs:label "Removal of the Range" .


###  https://w3id.orgdef/och#RemoveReflexiveObjectProperty
<https://w3id.orgdef/och#RemoveReflexiveObjectProperty> rdf:type owl:Class ;
                                                        rdfs:subClassOf <https://w3id.orgdef/och#ReflexiveObjectPropertyChange> ,
                                                                        <https://w3id.orgdef/och#RemoveObjectProperty> ;
                                                        rdfs:comment "The class of the removal of the owl:reflexiveProperty change betweeen ontology versions.The class of rreflexive properties." ;
                                                        rdfs:label "Removal of an reflexive object property " .


###  https://w3id.orgdef/och#RemoveSubClass
<https://w3id.orgdef/och#RemoveSubClass> rdf:type owl:Class ;
                                         rdfs:subClassOf <https://w3id.orgdef/och#SubClassChange> ;
                                         rdfs:comment "The change operation that describes the removal of an rdfs:subClassOf property." ;
                                         rdfs:label "Removal of SubClass property" .


###  https://w3id.orgdef/och#RemoveSubPropertyOf
<https://w3id.orgdef/och#RemoveSubPropertyOf> rdf:type owl:Class ;
                                              rdfs:subClassOf <https://w3id.orgdef/och#SubPropertyChange> ;
                                              rdfs:comment "The change operation that describes the removal of sub property property." ;
                                              rdfs:label "Removal of the sub property property" .


###  https://w3id.orgdef/och#RemoveSymmetricObjectProperty
<https://w3id.orgdef/och#RemoveSymmetricObjectProperty> rdf:type owl:Class ;
                                                        rdfs:subClassOf <https://w3id.orgdef/och#RemoveObjectProperty> ,
                                                                        <https://w3id.orgdef/och#SymmetricObjectPropertyChange> ;
                                                        rdfs:comment "The class of the removal of symmetric properties change betweeen ontology versions" ;
                                                        rdfs:label "Removal of Symetric Object Property" .


###  https://w3id.orgdef/och#RemoveTransitiveObjectProperty
<https://w3id.orgdef/och#RemoveTransitiveObjectProperty> rdf:type owl:Class ;
                                                         rdfs:subClassOf <https://w3id.orgdef/och#RemoveObjectProperty> ,
                                                                         <https://w3id.orgdef/och#TransitiveObjectPropertyChange> ;
                                                         rdfs:comment "The change operation that describes the removal of a transitive object property." ;
                                                         rdfs:label "Removal of a transitive object property" .


###  https://w3id.orgdef/och#RenameElement
<https://w3id.orgdef/och#RenameElement> rdf:type owl:Class ;
                                        rdfs:subClassOf <https://w3id.orgdef/och#ElementChange> ;
                                        rdfs:comment "The change operation that describes the Renaming of a class or property." ;
                                        rdfs:label "Renaming of a class or property" .


###  https://w3id.orgdef/och#RevokeDeprecate
<https://w3id.orgdef/och#RevokeDeprecate> rdf:type owl:Class ;
                                          rdfs:subClassOf <https://w3id.orgdef/och#ElementChange> ;
                                          rdfs:comment "The change operation that describes the revoke deprecation of a class or property" ;
                                          rdfs:label "Revoke Deprecation of an Element." .


###  https://w3id.orgdef/och#SubClassChange
<https://w3id.orgdef/och#SubClassChange> rdf:type owl:Class ;
                                         rdfs:subClassOf <https://w3id.orgdef/och#ClassChange> ;
                                         rdfs:comment "The change operation that describes the change of an rdfs:subClassOf property." ;
                                         rdfs:label "Change of SubClass property" .


###  https://w3id.orgdef/och#SubPropertyChange
<https://w3id.orgdef/och#SubPropertyChange> rdf:type owl:Class ;
                                            rdfs:subClassOf <https://w3id.orgdef/och#PropertyChange> ;
                                            rdfs:comment "The change operation that describes the change of a subproperty property" ;
                                            rdfs:label "Change of a Subproperty Property" .


###  https://w3id.orgdef/och#SymmetricObjectPropertyChange
<https://w3id.orgdef/och#SymmetricObjectPropertyChange> rdf:type owl:Class ;
                                                        rdfs:subClassOf <https://w3id.orgdef/och#ObjectPropertyChange> ;
                                                        rdfs:comment "The change operation that describes the change of a symmetric object property property." ;
                                                        rdfs:label "Change of the symmetric object property property" .


###  https://w3id.orgdef/och#TransitiveObjectPropertyChange
<https://w3id.orgdef/och#TransitiveObjectPropertyChange> rdf:type owl:Class ;
                                                         rdfs:subClassOf <https://w3id.orgdef/och#ObjectPropertyChange> ;
                                                         rdfs:comment "The change operation that describes the change of a transitive object property property." ;
                                                         rdfs:label "Change of the transitive object property property" .


###  Generated by the OWL API (version 5.1.18) https://github.com/owlcs/owlapi/
